equiv for slice

theories/logrel/logrel_prim.v
@@ -18,7 +18,7 @@ Section logrel_prim.
   (*    ) trans. *)
 
   Definition transferred_memory_slice (trans : gmap Addr transaction) (i: VMID) (j:VMID): iProp Σ:=
-     ∃ mem , memory_pages (pages_in_trans (filter (λ kv, (kv.2.1.1.1.1 = i ∧ kv.2.1.1.1.2 = j) ∧ ¬(kv.2.2 = true ∧ kv.2.1.2 = Lending))%type trans)) mem.
+    big_sepFM trans (λ kv, (kv.2.1.1.1.1 = i ∧ kv.2.1.1.1.2 = j) ∧ ¬(kv.2.2 = true ∧ kv.2.1.2 = Lending)) (λ _ tran, (∃ mem , memory_pages tran.1.1.2 mem)%I).
 
   Definition retrievable_transaction_transferred_slice (trans : gmap Addr transaction) (i:VMID) (j: VMID) : iProp Σ :=
     (big_sepFM trans (λ kv, kv.2.1.1.1.1 = i ∧ kv.2.1.1.1.2 = j) (λ k v, k -{1/2}>re v.2 )%I) ∗
